%
%	This is the modified solution for Q11 supplied by Dominic Corbett
%
\subsection*{Solution 11}

\begin{itemize}

\item[(a)][DC]

Note that
\begin{align*}
	f ( z )
	&=
	\frac{ \pi \cos ( \pi z ) }{ \del{ 4 z + 3 i } \del{ 4 z - 3 i } \sin ( \pi z ) }
\intertext{so by the cover-up rule (\textit{HB28---1.3})}
	\Res ( f , - i \tfrac{3}{4} )
	&=
	\frac{ \pi \cos ( - \pi i \tfrac{3}{4} ) }{ 4 \del{ 4 ( - i \tfrac{3}{4} ) - 3 i } \sin ( - \pi i \tfrac{3}{4} ) }
	\\
	&=
	\frac{ \pi \cosh ( - \tfrac{3}{4} \pi ) }{ - 24 i^2 \sinh ( - \tfrac{3}{4} \pi ) }
	\\
	&=
	\underline{\underline{
	- \tfrac{ \pi }{ 24 } \coth ( \tfrac{3}{4} \pi )
	}}
\intertext{and}
	\Res ( f , i \tfrac{3}{4} )
	&=
	\frac{ \pi \cos ( \pi i \tfrac{3}{4} ) }{ 4 \del{ 4 ( i \tfrac{3}{4} ) + 3 i } \sin ( \pi i \tfrac{3}{4} ) }
	\\
	&=
	\frac{ \pi \cosh ( \tfrac{3}{4} \pi ) }{ 24 i^2 \sinh ( \tfrac{3}{4} \pi ) }
	\\
	&=
	\underline{\underline{
	- \tfrac{ \pi }{ 24 } \coth ( \tfrac{3}{4} \pi )
	}}
\intertext{and by the $ g/h $ rule (\textit{HB28---1.2})}
	\Res ( f , 0 )
	&=
	\frac{ \pi \cos ( \pi (0) ) }{ \del{ 4 (0) + 3 i } \del{ 4 (0) - 3 i } \pi \cos ( \pi (0) ) }
	\\
	&=
	\frac{ 1 }{ ( 3 i ) ( - 3 i ) }
	\\
	&=
	\underline{\underline{
	\tfrac{ 1 }{ 9 }
	}}
\end{align*}

\item[(b)][DC]

$ \phi ( n ) = \frac{1}{16 n^2 + 9} $ is an even function which is analytic on $ \Complex $ except for poles at the points $ \tfrac{3}{4} i $ and $ - \tfrac{3}{4} i $. Now, if $ S_N $ is the square contour with vertices at $ (N + \tfrac{1}{2})(\pm 1 \pm i) $, then its length is $ L = 4 ( 2 N + 1 ) $ and
\label{11b}
\begin{align*}
	\abs{\cot \pi z}
	&\leq
	2
	\;\;\;\text{for $ z \in S_N $ (\textit{HB30---4.2})}
\intertext{and since $ \abs{ z } \geq N + \frac{1}{2} $ for $ z \in S_N $, we have}
	\abs{ 16 z^2 + 9 }
	&\geq
	\abs{ \abs{ 16 z^2 } - \abs{ 9 } }
	\;\;\;(\textit{HB11---5.2})
	\\
	&=
	\abs{ 16 \abs{ z }^2 - 9 }
	\\
	&\geq
	\abs{ 16 ( N + \tfrac{1}{2} )^2 - 9 }
	\;\;\;\text{for $ z \in S_N $}
	\\
	\therefore
	\abs{ f ( z ) }
	=
	\abs{ \frac{ \pi \cot ( \pi z ) }{ 16 z^2 + 9 } }
	&\leq
	\frac{ 2 \pi }{ 16 ( N + \tfrac{1}{2} )^2 - 9 }
	=
	M
	\;\;\;\text{for $ z \in S_N $}
\intertext{Hence, by the Estimation Theorem,}
	\abs{ \int_{S_N} f ( z ) \dd z }
	&\leq
	\frac{ 2 \pi }{ 16 ( N + \tfrac{1}{2} )^2 - 9 } \cdot 4 ( 2 N + 1 ) ,
\intertext{which tends to $ 0 $ as $ N \to \infty $, that is}
	\lim_{N\to\infty} \int_{S_N} f ( z ) \dd z
	&=
	0
\intertext{It follows by \textit{HB30---4.1} that}
	\sum_{n=1}^\infty \frac{1}{16 n^2 + 9}
	&=
	- \tfrac{1}{2} \del{ \Res ( f , 0 ) + \Res ( f , - i \tfrac{3}{4} ) + \Res ( f , i \tfrac{3}{4} ) }
	\\
	&=
	- \tfrac{1}{2} \del{ \tfrac{ 1 }{ 9 } - \tfrac{ \pi }{ 24 } \coth ( \tfrac{3}{4} \pi ) - \tfrac{ \pi }{ 24 } \coth ( \tfrac{3}{4} \pi ) }
	\\
	&=
	\underline{\underline{
	\tfrac{ \pi }{ 24 } \coth ( \tfrac{3}{4} \pi ) - \tfrac{1}{18}
	}}
\end{align*}

\item[(c)][DC]

Since
\begin{align*}
	\sum_{n=-\infty}^\infty \frac{1}{16 n^2 + 9}
	&=
	\sum_{n=-\infty}^{-1} \frac{1}{16 n^2 + 9}
	+
	\frac{1}{16 (0)^2 + 9}
	+
	\sum_{n=1}^\infty \frac{1}{16 n^2 + 9}
	\\
	&=
	\sum_{n=\infty}^{1} \frac{1}{16 (-n)^2 + 9}
	+
	\frac{1}{9}
	+
	\sum_{n=1}^\infty \frac{1}{16 n^2 + 9}
	\\
	&=
	\frac{1}{9}
	+
	2 \sum_{n=1}^\infty \frac{1}{16 n^2 + 9}
	\;\;\hbox{(sum of positive reals indp't of order)}
\intertext{we can simply substitute in our result from part~(b) to give}
	\sum_{n=-\infty}^\infty \frac{1}{16 n^2 + 9}
	&=
	\frac{1}{9}
	+
	\tfrac{ 2 \pi }{ 24 } \coth ( \tfrac{3}{4} \pi ) - \tfrac{2}{18}
	\\
	&=
	\underline{\underline{
	\tfrac{ \pi }{ 12 } \coth ( \tfrac{3}{4} \pi )
	}}
	\;\;\;\textsc{qed}
\end{align*}

\end{itemize}
